src/Std/Data/DTreeMap/Raw/Slice.lean
@@ -52,8 +52,8 @@ public instance {α : Type u} {β : α → Type v} [Ord α] (cmp : α → α →
     Rco.Sliceable (Raw α β cmp) α (Internal.RcoSlice α β) where
   mkSlice carrier range := ⟨carrier.inner, range⟩
 
-public theorem toList_rco {α : Type u} {β : α → Type v} [Ord α] [TransOrd α] {t : Raw α β compare} {wf : t.WF} {lower_bound upper_bound : α} :
-  t[lower_bound...<upper_bound].toList = t.toList.filter (fun e => (compare e.fst lower_bound).isGE ∧ (compare e.fst upper_bound).isLT) := by
+public theorem toList_rco {α : Type u} {β : α → Type v} [Ord α] [TransOrd α] {t : Raw α β compare} {wf : t.WF} {lowerBound upperBound : α} :
+  t[lowerBound...<upperBound].toList = t.toList.filter (fun e => (compare e.fst lowerBound).isGE ∧ (compare e.fst upperBound).isLT) := by
   apply Internal.toList_rco
   . exact wf.out.ordered
 
@@ -61,9 +61,9 @@ public instance {α : Type u} {β : α → Type v} [Ord α] (cmp : α → α →
     Rcc.Sliceable (Raw α β cmp) α (Internal.RccSlice α β) where
   mkSlice carrier range := ⟨carrier.inner, range⟩
 
-public theorem toList_rcc {α : Type u} {β : α → Type v} [Ord α] [TransOrd α] {t : Raw α β compare} {wf : t.WF} {lower_bound upper_bound : α} :
-  t[lower_bound...=upper_bound].toList =
-    t.toList.filter (fun e => (compare e.fst lower_bound).isGE ∧ (compare e.fst upper_bound).isLE) := by
+public theorem toList_rcc {α : Type u} {β : α → Type v} [Ord α] [TransOrd α] {t : Raw α β compare} {wf : t.WF} {lowerBound upperBound : α} :
+  t[lowerBound...=upperBound].toList =
+    t.toList.filter (fun e => (compare e.fst lowerBound).isGE ∧ (compare e.fst upperBound).isLE) := by
   apply Internal.toList_rcc
   . exact wf.out.ordered
 
@@ -81,9 +81,9 @@ public instance {α : Type u} {β : α → Type v} [Ord α] (cmp : α → α →
     Roc.Sliceable (Raw α β cmp) α (Internal.RocSlice α β) where
   mkSlice carrier range := ⟨carrier.inner, range⟩
 
-public theorem toList_roc {α : Type u} {β : α → Type v} [Ord α] [TransOrd α] {t : Raw α β compare} {wf : t.WF} {lower_bound upper_bound : α} :
-  t[lower_bound<...=upper_bound].toList =
-    t.toList.filter (fun e => (compare e.fst lower_bound).isGT ∧ (compare e.fst upper_bound).isLE) := by
+public theorem toList_roc {α : Type u} {β : α → Type v} [Ord α] [TransOrd α] {t : Raw α β compare} {wf : t.WF} {lowerBound upperBound : α} :
+  t[lowerBound<...=upperBound].toList =
+    t.toList.filter (fun e => (compare e.fst lowerBound).isGT ∧ (compare e.fst upperBound).isLE) := by
   apply Internal.toList_roc
   . exact wf.out.ordered
 
@@ -91,9 +91,9 @@ public instance {α : Type u} {β : α → Type v} [Ord α] (cmp : α → α →
     Roo.Sliceable (Raw α β cmp) α (Internal.RooSlice α β) where
   mkSlice carrier range := ⟨carrier.inner, range⟩
 
-public theorem toList_roo {α : Type u} {β : α → Type v} [Ord α] [TransOrd α] {t : Raw α β compare} {wf : t.WF} {lower_bound upper_bound : α} :
-  t[lower_bound<...upper_bound].toList =
-    t.toList.filter (fun e => (compare e.fst lower_bound).isGT ∧ (compare e.fst upper_bound).isLT) := by
+public theorem toList_roo {α : Type u} {β : α → Type v} [Ord α] [TransOrd α] {t : Raw α β compare} {wf : t.WF} {lowerBound upperBound : α} :
+  t[lowerBound<...upperBound].toList =
+    t.toList.filter (fun e => (compare e.fst lowerBound).isGT ∧ (compare e.fst upperBound).isLT) := by
   apply Internal.toList_roo
   . exact wf.out.ordered
 
